@prefix rdf: <http://www.w3.org/1999/02/22-rdf-syntax-ns#>.
@prefix rdfs: <http://www.w3.org/2000/01/rdf-schema#>.
@prefix xsd: <http://www.w3.org/2001/XMLSchema#>.
@prefix owl: <http://www.w3.org/2002/07/owl#>.
@prefix dc: <http://purl.org/dc/elements/1.1/>.
@prefix dcterms: <http://purl.org/dc/terms/>.
@prefix dwc: <http://rs.tdwg.org/dwc/terms/>.
@prefix skos: <http://www.w3.org/2004/02/skos/core#>.
@prefix tdwgutility: <http://rs.tdwg.org/dwc/terms/attributes/>.
@prefix foaf: <http://xmlns.com/foaf/0.1/>.
@prefix dwciri: <http://rs.tdwg.org/dwc/iri/>.

<http://rs.tdwg.org/dwcem/values/e>
     rdfs:isDefinedBy <http://rs.tdwg.org/dwcem/values/>;
     dcterms:isPartOf <http://rs.tdwg.org/dwcem/values/>;
     dcterms:created "2020-10-13"^^xsd:date;
     dcterms:modified "2020-10-13"^^xsd:date;
     rdfs:label "establishmentMeans controlled concept scheme"@en;
     skos:prefLabel "establishmentMeans controlled concept scheme"@en;
     rdfs:comment "A SKOS Concept Scheme to be used as a controlled vocabulary for the Darwin Core terms dwc:establishmentMeans and dwciri:establishmentMeans"@en;
     skos:definition "A SKOS Concept Scheme to be used as a controlled vocabulary for the Darwin Core terms dwc:establishmentMeans and dwciri:establishmentMeans"@en;
     rdf:type <http://www.w3.org/2004/02/skos/core#ConceptScheme> ;
     skos:hasTopConcept <http://rs.tdwg.org/dwcem/values/e001> , <http://rs.tdwg.org/dwcem/values/e002> , <http://rs.tdwg.org/dwcem/values/e003> , <http://rs.tdwg.org/dwcem/values/e004> , <http://rs.tdwg.org/dwcem/values/e005> , <http://rs.tdwg.org/dwcem/values/e006> .

<http://rs.tdwg.org/dwcem/values/version/e-2020-10-13>
     dcterms:isVersionOf <http://rs.tdwg.org/dwcem/values/e>.

<http://rs.tdwg.org/dwcem/values/e>
     dcterms:hasVersion <http://rs.tdwg.org/dwcem/values/version/e-2020-10-13>.

<http://rs.tdwg.org/dwcem/values/e.ttl>
     dc:format "text/turtle";
     dc:creator "Biodiversity Information Standards (TDWG)";
     dcterms:references <http://rs.tdwg.org/dwcem/values/e>;
     dcterms:modified "2020-10-17T11:10:09-04:00"^^xsd:dateTime;
     a foaf:document.

<http://rs.tdwg.org/dwcem/values/e001>
     rdfs:isDefinedBy <http://rs.tdwg.org/dwcem/values/>;
     dcterms:isPartOf <http://rs.tdwg.org/dwcem/values/>;
     dcterms:created "2020-10-13"^^xsd:date;
     dcterms:modified "2021-09-01"^^xsd:date;
     rdfs:label "native (indigenous)"@en;
     skos:prefLabel "native (indigenous)"@en;
     rdfs:comment "A taxon occurring within its natural range."@en;
     skos:definition "A taxon occurring within its natural range."@en;
     dcterms:description "What is considered native to an area varies with the biogeographic history of an area and the local interpretation of what is a \"natural range\"."@en;
     rdf:value "native";
     skos:inScheme <http://rs.tdwg.org/dwcem/values/e>;
     rdf:type <http://www.w3.org/2004/02/skos/core#Concept>.

<http://rs.tdwg.org/dwcem/values/version/e001-2020-10-13>
     dcterms:isVersionOf <http://rs.tdwg.org/dwcem/values/e001>.

<http://rs.tdwg.org/dwcem/values/e001>
     dcterms:hasVersion <http://rs.tdwg.org/dwcem/values/version/e001-2020-10-13>.

<http://rs.tdwg.org/dwcem/values/version/e001-2021-09-01>
     dcterms:isVersionOf <http://rs.tdwg.org/dwcem/values/e001>.

<http://rs.tdwg.org/dwcem/values/e001>
     dcterms:hasVersion <http://rs.tdwg.org/dwcem/values/version/e001-2021-09-01>.

<http://rs.tdwg.org/dwcem/values/e001.ttl>
     dc:format "text/turtle";
     dc:creator "Biodiversity Information Standards (TDWG)";
     dcterms:references <http://rs.tdwg.org/dwcem/values/e001>;
     dcterms:modified "2021-09-01T22:18:44-05:00"^^xsd:dateTime;
     a foaf:document.

<http://rs.tdwg.org/dwcem/values/e002>
     rdfs:isDefinedBy <http://rs.tdwg.org/dwcem/values/>;
     dcterms:isPartOf <http://rs.tdwg.org/dwcem/values/>;
     dcterms:created "2020-10-13"^^xsd:date;
     dcterms:modified "2021-09-01"^^xsd:date;
     rdfs:label "native: reintroduced"@en;
     skos:prefLabel "native: reintroduced"@en;
     rdfs:comment "A taxon re-established by direct introduction by humans into an area that was once part of its natural range, but from where it had become extinct."@en;
     skos:definition "A taxon re-established by direct introduction by humans into an area that was once part of its natural range, but from where it had become extinct."@en;
     dcterms:description "Where a taxon has become extirpated from an area where it had naturally occurred it may be returned to that area deliberately with the intension of re-establishing it."@en;
     rdf:value "nativeReintroduced";
     skos:inScheme <http://rs.tdwg.org/dwcem/values/e>;
     rdf:type <http://www.w3.org/2004/02/skos/core#Concept>.

<http://rs.tdwg.org/dwcem/values/version/e002-2020-10-13>
     dcterms:isVersionOf <http://rs.tdwg.org/dwcem/values/e002>.

<http://rs.tdwg.org/dwcem/values/e002>
     dcterms:hasVersion <http://rs.tdwg.org/dwcem/values/version/e002-2020-10-13>.

<http://rs.tdwg.org/dwcem/values/version/e002-2021-09-01>
     dcterms:isVersionOf <http://rs.tdwg.org/dwcem/values/e002>.

<http://rs.tdwg.org/dwcem/values/e002>
     dcterms:hasVersion <http://rs.tdwg.org/dwcem/values/version/e002-2021-09-01>.

<http://rs.tdwg.org/dwcem/values/e002.ttl>
     dc:format "text/turtle";
     dc:creator "Biodiversity Information Standards (TDWG)";
     dcterms:references <http://rs.tdwg.org/dwcem/values/e002>;
     dcterms:modified "2021-09-01T22:18:44-05:00"^^xsd:dateTime;
     a foaf:document.

<http://rs.tdwg.org/dwcem/values/e003>
     rdfs:isDefinedBy <http://rs.tdwg.org/dwcem/values/>;
     dcterms:isPartOf <http://rs.tdwg.org/dwcem/values/>;
     dcterms:created "2020-10-13"^^xsd:date;
     dcterms:modified "2021-09-01"^^xsd:date;
     rdfs:label "introduced (alien, exotic, non-native, nonindigenous)"@en;
     skos:prefLabel "introduced (alien, exotic, non-native, nonindigenous)"@en;
     rdfs:comment "Establishment of a taxon by human agency into an area that is not part of its natural range."@en;
     skos:definition "Establishment of a taxon by human agency into an area that is not part of its natural range."@en;
     dcterms:description "Organisms can be introduced to novel areas and habitats by human activity, either on purpose or by accident. Humans can also inadvertently create corridors that break down natural barriers to dispersal and allow organisms to spread beyond their natural range."@en;
     rdf:value "introduced";
     skos:inScheme <http://rs.tdwg.org/dwcem/values/e>;
     rdf:type <http://www.w3.org/2004/02/skos/core#Concept>.

<http://rs.tdwg.org/dwcem/values/version/e003-2020-10-13>
     dcterms:isVersionOf <http://rs.tdwg.org/dwcem/values/e003>.

<http://rs.tdwg.org/dwcem/values/e003>
     dcterms:hasVersion <http://rs.tdwg.org/dwcem/values/version/e003-2020-10-13>.

<http://rs.tdwg.org/dwcem/values/version/e003-2021-09-01>
     dcterms:isVersionOf <http://rs.tdwg.org/dwcem/values/e003>.

<http://rs.tdwg.org/dwcem/values/e003>
     dcterms:hasVersion <http://rs.tdwg.org/dwcem/values/version/e003-2021-09-01>.

<http://rs.tdwg.org/dwcem/values/e003.ttl>
     dc:format "text/turtle";
     dc:creator "Biodiversity Information Standards (TDWG)";
     dcterms:references <http://rs.tdwg.org/dwcem/values/e003>;
     dcterms:modified "2021-09-01T22:18:44-05:00"^^xsd:dateTime;
     a foaf:document.

<http://rs.tdwg.org/dwcem/values/e004>
     rdfs:isDefinedBy <http://rs.tdwg.org/dwcem/values/>;
     dcterms:isPartOf <http://rs.tdwg.org/dwcem/values/>;
     dcterms:created "2020-10-13"^^xsd:date;
     dcterms:modified "2021-09-01"^^xsd:date;
     rdfs:label "introduced: assisted colonisation"@en;
     skos:prefLabel "introduced: assisted colonisation"@en;
     rdfs:comment "Establishment of a taxon specifically with the intention of creating a self-sustaining wild population in an area that is not part of the taxon's natural range."@en;
     skos:definition "Establishment of a taxon specifically with the intention of creating a self-sustaining wild population in an area that is not part of the taxon's natural range."@en;
     dcterms:description "In the event of environmental change and habitat destruction a conservation option is to introduce a taxon into an area it did not naturally occur."@en;
     rdf:value "introducedAssistedColonisation";
     skos:inScheme <http://rs.tdwg.org/dwcem/values/e>;
     rdf:type <http://www.w3.org/2004/02/skos/core#Concept>.

<http://rs.tdwg.org/dwcem/values/version/e004-2020-10-13>
     dcterms:isVersionOf <http://rs.tdwg.org/dwcem/values/e004>.

<http://rs.tdwg.org/dwcem/values/e004>
     dcterms:hasVersion <http://rs.tdwg.org/dwcem/values/version/e004-2020-10-13>.

<http://rs.tdwg.org/dwcem/values/version/e004-2021-09-01>
     dcterms:isVersionOf <http://rs.tdwg.org/dwcem/values/e004>.

<http://rs.tdwg.org/dwcem/values/e004>
     dcterms:hasVersion <http://rs.tdwg.org/dwcem/values/version/e004-2021-09-01>.

<http://rs.tdwg.org/dwcem/values/e004.ttl>
     dc:format "text/turtle";
     dc:creator "Biodiversity Information Standards (TDWG)";
     dcterms:references <http://rs.tdwg.org/dwcem/values/e004>;
     dcterms:modified "2021-09-01T22:18:44-05:00"^^xsd:dateTime;
     a foaf:document.

<http://rs.tdwg.org/dwcem/values/e005>
     rdfs:isDefinedBy <http://rs.tdwg.org/dwcem/values/>;
     dcterms:isPartOf <http://rs.tdwg.org/dwcem/values/>;
     dcterms:created "2020-10-13"^^xsd:date;
     dcterms:modified "2020-10-13"^^xsd:date;
     rdfs:label "vagrant (casual)"@en;
     skos:prefLabel "vagrant (casual)"@en;
     rdfs:comment "The temporary occurrence of a taxon far outside its natural or migratory range."@en;
     skos:definition "The temporary occurrence of a taxon far outside its natural or migratory range."@en;
     dcterms:description "Natural events and human activity can disperse organisms unpredictably into places where they may stay or survive for a period."@en;
     rdf:value "vagrant";
     skos:inScheme <http://rs.tdwg.org/dwcem/values/e>;
     rdf:type <http://www.w3.org/2004/02/skos/core#Concept>.

<http://rs.tdwg.org/dwcem/values/version/e005-2020-10-13>
     dcterms:isVersionOf <http://rs.tdwg.org/dwcem/values/e005>.

<http://rs.tdwg.org/dwcem/values/e005>
     dcterms:hasVersion <http://rs.tdwg.org/dwcem/values/version/e005-2020-10-13>.

<http://rs.tdwg.org/dwcem/values/e005.ttl>
     dc:format "text/turtle";
     dc:creator "Biodiversity Information Standards (TDWG)";
     dcterms:references <http://rs.tdwg.org/dwcem/values/e005>;
     dcterms:modified "2020-10-17T11:10:09-04:00"^^xsd:dateTime;
     a foaf:document.

<http://rs.tdwg.org/dwcem/values/e006>
     rdfs:isDefinedBy <http://rs.tdwg.org/dwcem/values/>;
     dcterms:isPartOf <http://rs.tdwg.org/dwcem/values/>;
     dcterms:created "2020-10-13"^^xsd:date;
     dcterms:modified "2021-09-01"^^xsd:date;
     rdfs:label "uncertain (unknown, cryptogenic)"@en;
     skos:prefLabel "uncertain (unknown, cryptogenic)"@en;
     rdfs:comment "The origin of the occurrence of the taxon in an area is obscure."@en;
     skos:definition "The origin of the occurrence of the taxon in an area is obscure."@en;
     dcterms:description "When there is a lack of fossil or historical evidence for the occurrence of a taxon in an area it can be impossible to know if the taxon is new to the area or native."@en;
     rdf:value "uncertain";
     skos:inScheme <http://rs.tdwg.org/dwcem/values/e>;
     rdf:type <http://www.w3.org/2004/02/skos/core#Concept>.

<http://rs.tdwg.org/dwcem/values/version/e006-2020-10-13>
     dcterms:isVersionOf <http://rs.tdwg.org/dwcem/values/e006>.

<http://rs.tdwg.org/dwcem/values/e006>
     dcterms:hasVersion <http://rs.tdwg.org/dwcem/values/version/e006-2020-10-13>.

<http://rs.tdwg.org/dwcem/values/version/e006-2021-09-01>
     dcterms:isVersionOf <http://rs.tdwg.org/dwcem/values/e006>.

<http://rs.tdwg.org/dwcem/values/e006>
     dcterms:hasVersion <http://rs.tdwg.org/dwcem/values/version/e006-2021-09-01>.

<http://rs.tdwg.org/dwcem/values/e006.ttl>
     dc:format "text/turtle";
     dc:creator "Biodiversity Information Standards (TDWG)";
     dcterms:references <http://rs.tdwg.org/dwcem/values/e006>;
     dcterms:modified "2021-09-01T22:18:44-05:00"^^xsd:dateTime;
     a foaf:document.

